---
id: 220
title: 圆锥曲线
question_type: 圆方程
domain: 高中数学竞赛几何
difficulty: 中学
knowledge_point: 圆方程
batch: 01_第一批100题
teacher: sunjingxuan
---

## 题目
Determine the slope of the other common external tangent line that passes through the origin, given that in a Cartesian coordinate system, two circles have a common point at $(9,6)$, both are tangent to the x-axis, and the product of their radius is 68.

## 解答
Step 1: Since the line connecting the centers of the two circles passes through the origin, we can denote the centers of the two circles as $(a, ka)$ and $(b, kb)$, where $k$ represents the slope of the line through the origin.  
Step 2: For the first circle with center $(a, ka)$, the distance from its center to the point $(9, 6)$ must equal its radius. This gives the equation $(a - 9)^2 + (ka - 6)^2 = (ka)^2$. Expanding the left-hand side, we obtain $a^2 - 18a + 81 + k^2a^2 - 12ka + 36 = k^2a^2$. Simplifying by canceling $k^2a^2$ from both sides and combining like terms, we get $a^2 - 18a + 117 - 12ka = 0$. Rearranging terms to form a quadratic equation in $a$, we have $a^2 - 6(2k + 3)a + 117 = 0$.  
Step 3: Similarly, for the second circle with center $(b, kb)$, applying the same distance condition to the point $(9, 6)$ yields $(b - 9)^2 + (kb - 6)^2 = (kb)^2$. Expanding and simplifying this equation as in Step 2 results in $b^2 - 6(2k + 3)b + 117 = 0$.  
Step 4: Since $a \neq b$, both $a$ and $b$ are distinct roots of the quadratic equation $x^2 - 6(2k + 3)x + 117 = 0$. By Vieta's formulas, the product of the roots $ab$ is equal to the constant term of the quadratic, so $ab = 117$.  
Step 5: The product of the $y$-coordinates of the centers is $ka \cdot kb = k^2ab$. We are given that this product equals 68, so $k^2ab = 68$. Substituting $ab = 117$ from Step 4, we obtain $k^2 \cdot 117 = 68$. Solving for $k^2$, we find $k^2 = \frac{68}{117}$, and thus $k = \sqrt{\frac{68}{117}} = \frac{2\sqrt{17}}{3\sqrt{13}}$ (after rationalizing the denominator).  
Step 6: The slope of the other external common tangent is given by the formula $\frac{2k}{1 - k^2}$. Substituting $k^2 = \frac{68}{117}$, we first calculate the denominator: $1 - \frac{68}{117} = \frac{117 - 68}{117} = \frac{49}{117}$. Then the slope becomes $\frac{2k}{\frac{49}{117}} = 2k \cdot \frac{117}{49}$. Substituting $k = \frac{2\sqrt{17}}{3\sqrt{13}}$, we get $2 \cdot \frac{2\sqrt{17}}{3\sqrt{13}} \cdot \frac{117}{49} = \frac{4\sqrt{17} \cdot 117}{3\sqrt{13} \cdot 49}$. Simplifying $\frac{117}{3} = 39$, this reduces to $\frac{4\sqrt{17} \cdot 39}{\sqrt{13} \cdot 49} = \frac{156\sqrt{17}}{49\sqrt{13}}$. Rationalizing the denominator by multiplying the numerator and denominator by $\sqrt{13}$, we obtain $\frac{156\sqrt{17} \cdot \sqrt{13}}{49 \cdot 13} = \frac{156\sqrt{221}}{637}$. Since $\frac{156}{13} = 12$, this simplifies to $\frac{12\sqrt{221}}{49}$.

## 答案
$$\frac{12\sqrt{221}}{49}$$
